Validator/Hedge.lean
@@ -1,3 +1,4 @@
 import Validator.Hedge.Grammar
 import Validator.Hedge.IfExpr
 import Validator.Hedge.Language
+import Validator.Hedge.Types
