Validator/Hedge/Types.lean
@@ -1,0 +1,45 @@
+import Validator.Regex.Regex
+
+-- ## Definition 3.2.3: Regular Hedge Grammar
+--   𝐺 = (𝑁, 𝑇, 𝑆, 𝑃)
+--   𝑁 a finite set of non-terminals
+--   𝑇 a finite set of terminals
+--   𝑆 the start symbol of a regular hedge grammar is a regular expression comprising pairs of nonterminals and terminals (a regular expression over N × T)
+--   𝑃 a set of production rules of a regular hedge grammar are of the form X → r such that r is a regular expression over N × T.
+
+namespace Hedge.Grammar
+
+-- Ref is a non-terminal, where n represents the number of non-terminals
+abbrev Ref (n: Nat) := Fin n
+
+abbrev Symbol (n: Nat) (φ: Type) := (φ × Ref n)
+
+abbrev Symbols n φ l := Vec (Symbol n φ) l
+
+abbrev Rule (n: Nat) (φ: Type) := Regex (Symbol n φ)
+
+abbrev Rules (n: Nat) (φ: Type) (l: Nat) := Vec (Rule n φ) l
+
+end Hedge.Grammar
+
+namespace Hedge
+
+structure Grammar (n: Nat) (φ: Type) where
+  start: Hedge.Grammar.Rule n φ
+  prods: Vec (Hedge.Grammar.Rule n φ) n
+
+end Hedge
+
+namespace Hedge.Grammar
+
+def hashVector [Hashable α] (xs: Vec α n): UInt64 :=
+  hash xs.toList
+
+instance (α: Type) (n: Nat) [Hashable α] : Hashable (Vec α n) where
+  hash := hashVector
+
+def hashRules {n: Nat} {φ: Type} {l: Nat} [Hashable φ] (xs: Rules n φ l): UInt64 :=
+  hash xs.toList
+
+instance (n: Nat) (φ: Type) (l: Nat) [Hashable φ] : Hashable (Rules n φ l) where
+  hash := hashRules
